moving some code around, mostly tactics

src/compiler.v
@@ -2,11 +2,26 @@ Require Import ZArith.
 Local Open Scope Z_scope.
 
 Require Import String.
+Require Import List.
 Open Scope list_scope.
 
-Require Import wacket.
+Require Import language.definition.
+
 Require Import wasmLite.
-Require Import List.
+
+
+Definition uniOpToString op: string := match op with 
+| D_U_add1 => "add1"
+| D_U_sub1 => "sub1"
+| D_U_zero => "zero"
+| D_U_not => "not"
+end.
+
+Definition typeToString type: string := match type with 
+| D_type_Int => "Int"
+| D_type_Bool => "Bool"
+| D_type_Error => "Error"
+end.
 
 
 Inductive compilerResult : Type := 
@@ -14,69 +29,75 @@ Inductive compilerResult : Type :=
 | Error (err: string)
 .
 
-Definition typeSame t1 t2 := match (t1,t2) with 
-| (typ_Int,typ_Int) => true
-| (typ_Bool,typ_Bool) => true
-| (typ_Error,typ_Error) => true
-| _ => false
-end.
 
-Definition compileUniOp op := match op with 
-| D_U_add1 => (i64.const 1)::(i64.add)::nil
-| D_U_sub1 => (i64.const 1)::(i64.sub)::nil
-| D_U_zero => i64.eqz::nil
-| D_U_not => i32.eqz::nil
+Definition compileUniOp op t := match (op,t) with 
+| (D_U_add1,D_type_Int) => (i64.const 1)::(i64.add)::nil
+| (D_U_sub1,D_type_Int) => (i64.const 1)::(i64.sub)::nil
+| (D_U_zero,D_type_Int) => i64.eqz::nil
+| (D_U_not,D_type_Bool) => i32.eqz::nil
+| _ => nil
 end.
 
 Fixpoint compile_typed (source: dupe) := match source with 
-| D_Integer z => (typ_Int, Succ ((i64.const z)::nil))
-| D_Boolean b => (typ_Bool, Succ ((i32.const (if b then 1 else 0))::nil)) 
+| D_Integer z => (D_type_Int, Succ ((i64.const z)::nil))
+| D_Boolean b => (D_type_Bool, Succ ((i32.const (if b then 1 else 0))::nil)) 
 
 | D_UniOp op expr => 
     match compile_typed expr with 
     | (t, Succ code) => 
-        if typeSame t (uniOpExpectedType op) 
-        then (uniOpResultType op ,Succ (code ++ (compileUniOp op)))
-        else (typ_Error, Error (
-            (uniOpToString op) ++ "expression had type of: " ++ (typeToString t) ++
-            " expected type of : " ++ (typeToString (uniOpExpectedType op))
+        match uniOpTypeSignatureForAccept op t with 
+        | Some(accepts,returns) => (returns, Succ (code ++ (compileUniOp op accepts)) )
+        | None => (D_type_Error, Error (
+            (uniOpToString op) ++ "expression had invalid type of: " ++ (typeToString t)
         ))
-    | (_, (Error err)) => (typ_Error, Error err)
+        end
+    | (_, (Error err)) => (D_type_Error, Error err)
     end
 | D_if b t e => 
     match (compile_typed b, compile_typed t, compile_typed e) with 
-    | ((typ_Bool, Succ codeB),(t1, Succ codeT),(t2, Succ codeE)) =>
+    | ((D_type_Bool, Succ codeB),(t1, Succ codeT),(t2, Succ codeE)) =>
         if(typeSame t1 t2) 
         then (t1, Succ (codeB ++ (ifThenElse codeT codeE)::nil))
-        else (typ_Error, Error "if type mismatch")
-    | ((typ_Int, Succ codeB),(t1, Succ codeT),(t2, Succ codeE)) =>
+        else (D_type_Error, Error "if type mismatch")
+    | ((D_type_Int, Succ codeB),(t1, Succ codeT),(t2, Succ codeE)) =>
         if(typeSame t1 t2) 
         then (t1, Succ codeT)
-        else (typ_Error, Error "if type mismatch")
-    | ((_, Error err),(_, _),(_, _)) => (typ_Error, Error err)
-    | ((_, _),(_, Error err),(_, _)) => (typ_Error, Error err)
-    | ((_, _),(_, _),(_, Error err)) => (typ_Error, Error err)
-    | _ => (typ_Error, Error "unkown error")
+        else (D_type_Error, Error "if type mismatch")
+    | ((_, Error err),(_, _),(_, _)) => (D_type_Error, Error err)
+    | ((_, _),(_, Error err),(_, _)) => (D_type_Error, Error err)
+    | ((_, _),(_, _),(_, Error err)) => (D_type_Error, Error err)
+    | _ => (D_type_Error, Error "unkown error")
     end
 end.
-
 
 Definition compile (source :dupe) := match compile_typed source with 
 | (_,Succ code) => Succ code
 | (_,Error err) => Error err
 end.
 
+Lemma compileSucc_implies_typedSucc :
+forall src compiled, 
+    compile src = compiled ->
+    exists t, compile_typed src = (t,compiled).
+Proof.
+intros.
+unfold compile in H.
+destruct compiled; destruct (compile_typed src); destruct c;
+(try discriminate); exists d;rewrite H; reflexivity.
+Qed.
+
+
 Lemma uniaryOp_ImpliesSource:
 forall src compiled op, 
     compile (D_UniOp op src) = Succ compiled ->
-    exists code, ((compile src = Succ code) /\ (compiled = code ++ (compileUniOp op))).
+    exists code, ((compile src = Succ code) /\ (compiled = code ++ (compileUniOp op (typeOfDupe src)))).
 Proof.
    Admitted.
 
 Lemma ifBool_ImpliesSource :
-forall srcIf srcThen srcElse compiled b, 
+forall srcIf srcThen srcElse compiled, 
     compile (If srcIf Then srcThen Else srcElse) = Succ compiled ->
-    srcIf d==> (DR_Bool b)->
+    typeOfDupe srcIf = D_type_Bool ->
     exists codeIf codeThen codeElse, 
         ((compile srcIf = Succ codeIf) /\ (compile srcThen = Succ codeThen) /\ (compile srcElse = Succ codeElse) /\
         (compiled = codeIf ++ ((ifThenElse codeThen codeElse)::nil))).
@@ -85,9 +106,9 @@ Proof.
 
 
 Lemma ifInt_ImpliesSource :
-forall srcIf srcThen srcElse compiled z, 
+forall srcIf srcThen srcElse compiled, 
     compile (If srcIf Then srcThen Else srcElse) = Succ compiled ->
-    srcIf d==> (DR_Int z)->
+    typeOfDupe srcIf = D_type_Int->
     exists codeIf codeThen codeElse, 
         ((compile srcIf = Succ codeIf) /\ (compile srcThen = Succ codeThen) /\ (compile srcElse = Succ codeElse) /\
         (compiled = codeThen)).
