src/language/definition.v
@@ -1,10 +1,24 @@
 Require Import Bool List ZArith.
-Require Import String.
 
 Local Open Scope Z_scope.
 
 (* based on the dupe language 
 https://www.cs.umd.edu/class/spring2022/cmsc430/Dupe.html *)
+
+Inductive dupeType: Type :=
+| D_type_Int
+| D_type_Bool
+| D_type_Error
+.
+
+Definition typeSame t1 t2 := match (t1,t2) with 
+| (D_type_Int,D_type_Int) => true
+| (D_type_Bool,D_type_Bool) => true
+| (D_type_Error,D_type_Error) => true
+| _ => false
+end.
+
+
 
 Inductive dupeUniaryOp : Type :=
 | D_U_add1 
@@ -13,12 +27,29 @@ Inductive dupeUniaryOp : Type :=
 | D_U_not
 .
 
-Definition uniOpToString (u :dupeUniaryOp) : string := match u with 
-| D_U_add1 => "add1"
-| D_U_sub1 => "sub1"
-| D_U_zero => "zero?"
-| D_U_not => "!"
-end.
+Definition uniOpTypeSignature op := match op with 
+| D_U_add1 => (D_type_Int,D_type_Int)::nil
+| D_U_sub1 => (D_type_Int,D_type_Int)::nil
+| D_U_zero => (D_type_Int,D_type_Bool)::nil
+| D_U_not => (D_type_Bool,D_type_Bool)::nil
+end. 
+
+Definition uniOpAcceptsType op typ := 
+    let (accepts,returns) := split (uniOpTypeSignature op) in
+    In typ accepts
+. 
+
+Definition uniOpTypeSignatureForAccept op t := 
+    let signatureList := uniOpTypeSignature op in 
+    let fix search lst := match lst with 
+    | (accepts,returns)::tail => if typeSame accepts t 
+            then Some (accepts,returns)
+            else search tail 
+    | nil => None
+    end in search signatureList
+.
+
+
 
 Inductive dupe: Type :=
 | D_Integer: Z -> dupe
@@ -39,129 +70,6 @@ Notation "'(' 'Bool' b ')'" := (D_Boolean b).
 Notation "'(' 'Prim1' op exp ')'" := (D_UniOp op exp).
 Notation "'(' 'If' b 'Then' t 'Else' e ')'" := (D_if b t e).
 
-Inductive dupeType: Type :=
-| D_type_Int
-| D_type_Bool
-| D_type_Error
-.
-
-Definition typeSame t1 t2 := match (t1,t2) with 
-| (D_type_Int,D_type_Int) => true
-| (D_type_Bool,D_type_Bool) => true
-| (D_type_Error,D_type_Error) => true
-| _ => false
-end.
-
-
-Definition typeToString (t:dupeType) : string := match t with 
-| D_type_Int => "Int"
-| D_type_Bool => "Bool"
-| D_type_Error => "Error"
-end.
-
-Inductive dupeResult : Type :=
-| DR_Int: Z -> dupeResult
-| DR_Bool: bool -> dupeResult
-| DR_Error: dupeResult
-.
-
-Definition resultType result := match result with 
-| DR_Int _ => D_type_Int
-| DR_Bool _ => D_type_Bool
-| DR_Error => D_type_Error
-end.
-
-Definition uniOpTypeSignature op := match op with 
-| D_U_add1 => (D_type_Int,D_type_Int)::nil
-| D_U_sub1 => (D_type_Int,D_type_Int)::nil
-| D_U_zero => (D_type_Int,D_type_Bool)::nil
-| D_U_not => (D_type_Bool,D_type_Bool)::nil
-end. 
-
-Definition uniOpAcceptsType op typ := 
-    let (accepts,returns) := split (uniOpTypeSignature op) in
-    In typ accepts
-. 
-
-
-
-Definition uniOpTypeSignatureForAccept op t := 
-    let signatureList := uniOpTypeSignature op in 
-    let fix search lst := match lst with 
-    | (accepts,returns)::tail => if typeSame accepts t 
-            then Some (accepts,returns)
-            else search tail 
-    | nil => None
-    end in search signatureList
-.
-
-Definition uniOpTypeSignatureForReturn op t := 
-    let signatureList := uniOpTypeSignature op in 
-    let fix search lst := match lst with 
-    | (accepts,returns)::tail => if typeSame returns t 
-            then Some (accepts,returns)
-            else search tail 
-    | nil => None
-    end in search signatureList
-.
-
-Definition uniOpTransform op result := match (op, result) with 
-| (D_U_add1, DR_Int z) => DR_Int (z + 1)
-| (D_U_sub1, DR_Int z) => DR_Int (z - 1)
-| (D_U_zero, DR_Int z) => DR_Bool (z =? 0)
-| (D_U_not, DR_Bool b) => DR_Bool (negb b)
-| _ => DR_Error
-end.
-
-
-Fixpoint evalDupe(d : dupe) := match d with 
-| (D_Integer z) => (DR_Int z)
-| (D_Boolean b) => (DR_Bool b)
-| (D_UniOp op exp) => uniOpTransform op (evalDupe exp)
-| (D_if e1 e2 e3) => match (evalDupe e1, evalDupe e2, evalDupe e3) with 
-    | (DR_Bool b, res1, res2) => 
-        if (typeSame (resultType res1) (resultType res2)) && (negb (typeSame (resultType res1) D_type_Error))
-        then if b then res1 else res2
-        else DR_Error
-    | (DR_Int _, res1, res2 ) =>
-        if (typeSame (resultType res1) (resultType res2)) && (negb (typeSame (resultType res1) D_type_Error))
-        then res1
-        else DR_Error
-    | _ => DR_Error
-    end
-end.
-
-
-(* this will probably have to be changed because of how integers are represented in binary*)
-Reserved Notation " src 'd==>' val " (at level 50, left associativity).
-Inductive dupeEval: dupe -> (dupeType * dupeResult)%type -> Prop :=
-| E_D_Interger: forall z, (D_Integer z) d==> (D_type_Int, (DR_Int z))
-| E_D_Boolean: forall b, (D_Boolean b) d==> (D_type_Bool ,(DR_Bool b))
-
-| E_D_UniOp: forall t v inputType op evalType,
-    t d==> (inputType, v) ->
-    In (inputType, evalType) (uniOpTypeSignature op) ->
-    (D_UniOp op t) d==> (evalType,(uniOpTransform op v))
-
-| E_D_ifFalse: forall t_if t_then vt t_else ve evalType,
-    t_if d==> (D_type_Bool,(DR_Bool false)) -> 
-    t_then d==> (evalType,vt) ->
-    t_else d==> (evalType,ve) ->
-    (D_if t_if t_then t_else) d==> (evalType,ve)
-| E_D_ifTrue: forall t_if t_then vt t_else ve evalType,
-    t_if d==> (D_type_Bool,(DR_Bool true)) -> 
-    t_then d==> (evalType,vt) ->
-    t_else d==> (evalType,ve) ->
-    (D_if t_if t_then t_else) d==> (evalType,vt)
-| E_D_ifInt: forall t_if z t_then vt t_else ve evalType,
-    t_if d==> (D_type_Int,(DR_Int z)) -> 
-    t_then d==> (evalType,vt) ->
-    t_else d==> (evalType,ve) ->
-    (D_if t_if t_then t_else) d==> (evalType,vt)
-
-where " src 'd==>' val " := (dupeEval src val).
-
-
 Fixpoint typeOfDupe (source :dupe) := match source with 
 | D_Integer _ => D_type_Int
 | D_Boolean _ => D_type_Bool
@@ -178,245 +86,4 @@ Fixpoint typeOfDupe (source :dupe) := match source with
 end.
 
 
-Ltac evalPreamble := 
-try match goal with 
-| |- forall (src : dupe) (val : dupeResult), src d==> (resultType val, val) -> _ => 
-        induction src; intros
-| |- forall (src : dupe) (val : dupeResult), evalDupe src = val -> _ =>
-        induction src; intros; try (simpl in *; subst; constructor)
-end.
-
-Ltac destructDupeProperties := 
-repeat match goal with 
-| dUniop: dupeUniaryOp |- _ => 
-        destruct dUniop; simpl in *;(try discriminate)
-| dResult: dupeResult |- _ => 
-        destruct dResult; simpl in *;(try discriminate)
-| dType: dupeType |- _ => 
-        destruct dType; simpl in *;(try discriminate)
-end.
-
-Ltac refineHypothesis := 
-repeat match goal with 
-    | H : False |- _ => contradiction H
-    | H : _ \/ _ |- _ => destruct H
-    | H : _ /\ _ |- _ => destruct H
-    | H: ?a = ?a |- _ => clear H
-    | H: (_,_) = (_,_) |- _ => inversion H;subst
-    | H: context[In _ _] |- _ => simpl in H
-end.
-
-Ltac invertConstructiveDupe := 
-    match goal with 
-    | H: D_Integer ?z d==> (?type,?val) |- _ => inversion H; subst
-    | H: D_Boolean ?b d==> (?type,?val) |- _ => inversion H; subst
-    | H: (D_UniOp ?op ?src) d==> (?type,?val) |- _ => inversion H; subst
-    | H: (D_if ?srcIf ?srcThen ?srcElse) d==> (?type,?val) |- _ => inversion H; subst
-    end; (try reflexivity)
-.
-
-
-Theorem evalTypesSame:
-    forall src type val,
-        src d==> (type, val) ->
-        resultType val = type.
-Proof. 
-    induction src; intros;
-    evalPreamble;
-    destructDupeProperties;
-    invertConstructiveDupe;
-    refineHypothesis; (try discriminate);
-    repeat match goal with 
-    | H : ?src d==> (?type, ?val),
-        IH: forall (type : dupeType) (val : dupeResult),
-        ?src d==> (type, val) -> resultType val = type 
-        |- _ =>
-        specialize (IH type val H); subst
-    end; 
-    destructDupeProperties;
-    try reflexivity.
-Qed.
-
-Ltac removeSpecificType := 
-match goal with 
-| |- forall (src : dupe) (type : dupeType) (val : dupeResult), src d==> (type, val) -> _ => 
-    intros; let tmp := fresh "H" in 
-    let eq := fresh "eq" in
-    match goal with 
-    | H: ?src d==> (?type, ?val) |- _ => 
-        remember H as tmp eqn: eq; clear eq;
-        apply evalTypesSame in tmp;
-        rewrite <- tmp in *; (try discriminate);
-        clear tmp; clear type;
-        generalize dependent val;
-        generalize dependent src
-    end
-| H: ?src d==> (?type, ?val) |- _ => 
-    lazymatch goal with 
-    | H1: ?src1 d==> (type, ?val1),
-        H2: resultType ?val1 = type |- _ => fail
-    | H1: resultType val = type |- _ => fail
-    | |- _ => let tmp := fresh "H" in 
-        let eq := fresh "eq" in
-        remember H as tmp eqn: eq; clear eq;
-        apply evalTypesSame in tmp; 
-        rewrite <- tmp in *; (try discriminate)
-    end
-end.
-
-Ltac specializeIH := match goal with 
-| IH: ?hyp -> ?prop, H: ?hyp |- _ => specialize (IH H)
-
-| H: ?src d==> (?type, ?val),
-    IH: forall val : dupeResult, 
-    ?src d==> (resultType val, val) -> _ |- _ =>
-
-    let tmp := fresh "H" in 
-    let eq := fresh "eq" in
-    remember H as tmp eqn: eq; clear eq;
-    specialize (IH val);
-    eapply evalTypesSame in tmp; rewrite tmp in IH;
-    specialize (IH H);
-    clear tmp
-
-| IH: forall val: dupeResult,
-    evalDupe ?src = val -> _ |- _ => specialize (IH (evalDupe src))
-
-| H: ?src d==> (resultType ?val, ?val),
-    IH: forall (val: dupeResult),
-    ?src d==> (resultType val, val) -> _ |- _ => specialize (IH val H)
-
-| IH: ?a = ?a -> _ |- _ => 
-    let tmp := fresh "H" in 
-    assert (a = a) as tmp;[reflexivity | (specialize (IH tmp));clear tmp]
-
-| IH: (?t1 <> ?t2) -> _ |-  _ => 
-    let tmp := fresh "H" in 
-    assert (t1 <> t2) as tmp;[
-        solve[discriminate]|
-        specialize (IH tmp); clear tmp
-    ]
-end.
-
-Ltac applyEvalRules := 
-match goal with 
-    | |- (D_UniOp ?op ?src) d==> (?type, uniOpTransform ?op ?srcResult) => 
-        apply (E_D_UniOp src srcResult (resultType srcResult) op type); simpl;[
-            solve [try specializeIH; (try assumption)]| 
-            solve[(try contradiction);repeat ((left; reflexivity) || right)]
-        ]
-    | Hsrc1: ?src1 d==> (D_type_Int, DR_Int ?z),
-        Hsrc2: ?src2 d==> (?evalType, ?valThen),
-        Hsrc3: ?src3 d==> (?evalType, ?valElse)
-        |- (D_if ?src1 ?src2 ?src3) d==> (?evalType, ?valThen) => 
-            apply (E_D_ifInt src1 z src2 valThen src3 valElse evalType); assumption
-    | Hsrc1: ?src1 d==> (D_type_Bool, DR_Bool ?b),
-        Hsrc2: ?src2 d==> (?evalType, ?valThen),
-        Hsrc3: ?src3 d==> (?evalType, ?valElse)
-        |- (D_if ?src1 ?src2 ?src3) d==> (?evalType, if ?b then ?valThen else ?valElse) => 
-            destruct b; simpl; [
-                apply (E_D_ifTrue src1 src2 valThen src3 valElse evalType); assumption
-                | apply (E_D_ifFalse src1 src2 valThen src3 valElse evalType); assumption
-            ]  
-end.
-
-Ltac copyHypothesis H := 
-    let tmp := fresh "H" in 
-    let eq := fresh "eq" in
-    remember H as tmp eqn: eq; clear eq
-.
-
-Ltac rewriteLeft := match goal with 
-| H: ?l = _ |- context[?l] => rewrite -> H
-| H: ?l = _, H0: context[?l] |- _ => rewrite -> H in H0
-| _ => fail
-end.
-Ltac rewriteRight := match goal with 
-| H: _ = ?r |- context[?r] => rewrite <- H
-| H: _ = ?r, H0: context[?r] |- _ => rewrite <- H in H0
-| _ => fail
-end.
-
-
-Ltac evalAuto := 
-    try removeSpecificType;
-    evalPreamble;
-    destructDupeProperties;
-    try invertConstructiveDupe;
-    refineHypothesis; (try discriminate);
-    destructDupeProperties;
-    repeat removeSpecificType;
-    repeat specializeIH; repeat rewriteLeft;
-    (try reflexivity);
-    repeat match goal with 
-    | IH : resultType (evalDupe ?src) <> D_type_Error ->
-            ?src d==> (resultType (evalDupe ?src), evalDupe ?src)
-        |- _ => destruct (evalDupe src); simpl in IH; (try discriminate)
-    end;
-    repeat specializeIH;
-    try match goal with 
-    | H: _ = ?val |- _ d==> (_,?val) => rewrite <- H in *
-    end;
-    (simpl in *);
-    (try discriminate);
-    try applyEvalRules;
-    try match goal with 
-    | H: (if ?b then _ else _) = _ |- _=> destruct b; discriminate
-    | H: D_type_Error <> D_type_Error |- _ => contradiction
-    end
-.
-
-
-Theorem TypeOfDupe_same_as_Eval:
-    forall src type val,
-        src d==> (type, val) -> 
-        typeOfDupe src = type.
-Proof.
-    evalAuto.
-Qed.
-    
-
-Theorem evalDupe_implies_dupeEval: 
-    forall src val,
-    evalDupe src = val ->
-    ((resultType val) <> D_type_Error) ->
-    src d==> (resultType val, val).
-Proof.
-    evalAuto.
-Qed.
-
-
-Theorem dupeEval_implies_evalDupe: 
-    forall src val,
-    src d==> (resultType val, val) ->
-    evalDupe src = val.
-Proof.
-    evalAuto.
-Qed.
-
-
-Theorem dupeNotEvalError:
-forall src val,
-    src d==> (resultType val, val) ->
-    ((resultType val) <> D_type_Error).
-Proof.
-    evalAuto.
-Qed.
-
-
-Theorem evalEquivalence: 
-    forall src val,
-    src d==> (resultType val, val) <-> ((evalDupe src = val) /\ ((resultType val) <> D_type_Error)).
-Proof.
-    intros. 
-    split.
-    - split.
-        + apply dupeEval_implies_evalDupe. assumption.
-        + apply (dupeNotEvalError src). assumption.
-    - intros. 
-        destruct H.
-        apply  evalDupe_implies_dupeEval.
-        + assumption.
-        + assumption.
-Qed.
 
