src/ewacket.v
@@ -1,7 +1,9 @@
 Require Import Arith Bool List ZArith.
 Local Open Scope Z_scope.
 
-Require Import wacket.
+Require Import language.definition.
+Require Import language.eval.
+
 Require Import wasmLite.
 Require Import compiler.
 Require Import utils.
@@ -9,7 +11,7 @@ Require Import helperTactics.
 
 
 
-Definition dupeResult_to_wasmVal (res: dupeResult) :=
+Definition dupeResult_to_wasmVal res :=
 match res with 
 | DR_Int z => v_i64 z
 | DR_Bool b => if b then v_i32 1 else v_i32 0
@@ -20,57 +22,21 @@ Ltac applyInstructionOrder :=
 eapply instruction_order;
 eauto.
 
-Ltac unfoldCommon :=
-unfold testopOperation in *;
-unfold binopOperation in *;
-unfold UniOpTransform in *
-.
+
 
 Ltac unfoldCompiled H :=
     unfold compile in H; 
     simpl in H;
     inversion H. 
 
-Ltac stepCompletes := (
-    reflexivity || 
-    (apply Z.eqb_neq;reflexivity)
-).
 
-Ltac doesSingleStep := 
-    ( (eapply W_ST_64Const; stepCompletes)
-    || (eapply W_ST_32Const; stepCompletes)
-    || (eapply W_ST_inn_ibinop; stepCompletes)
-    || (eapply W_ST_inn_itestop; stepCompletes)
-    || (eapply W_ST_64IfTrue; stepCompletes)
-    || (eapply W_ST_64IfFalse; stepCompletes)
-    || (eapply W_ST_32IfTrue; stepCompletes)
-    || (eapply W_ST_32IfFalse; stepCompletes)
-    || (eapply W_ST_nop; stepCompletes)
-    || (eapply W_ST_unreachable; stepCompletes)
-    )
-.
-
-Ltac doesStep :=
-repeat (
-    unfoldCommon;
-    simpl in *;
-    (repeat destructBools);
-    (repeat removeListNils); 
-    (try assumption);
-    (try discriminate);
-    match goal with 
-    | [|- _ w-->* _ ]=> econstructor
-    | [|- multi wasmStepInd _ _] => econstructor
-    | [|- _ w--> _] => doesSingleStep
-    end
-).
 
 
 Ltac solveCase := 
-    repeat logicAuto;
+    repeat refineHypothesis;
     unfoldCommon;
     simpl in *;
-    (repeat refineInductiveHypothesis);
+    (repeat specializeIH);
     subst;
     (try applyInstructionOrder);
     (try doesStep);
@@ -83,9 +49,9 @@ Ltac solveCase :=
 and therefor evalDupe cannot produce an error, 
 honestly this should be a feature of the compiler*)
 Theorem semanticPreservation:
-    forall source compiled dupeResult,
+    forall source compiled dupeResult type,
     (compile source) = (Succ compiled) ->
-    source d==> dupeResult ->
+    source d==> (type, dupeResult) ->
     (compiled,nil) w-->* ((nil, (dupeResult_to_wasmVal dupeResult)::nil)).
 Proof.
     induction source; intros;
@@ -98,7 +64,13 @@ Proof.
         solveCase.
     (* uniary operators *)
     - apply uniaryOp_ImpliesSource in H.
-        destruct v; destruct d; (try discriminate); solveCase.
+        repeat destructDupeProperties;
+        repeat refineHypothesis; 
+        simpl in *; 
+        (try applyInstructionOrder).
+        doesStep.
+        
+        solveCase.
     (* if false*)
     - apply (ifBool_ImpliesSource source1 source2 source3 compiled #f) in H.
         + solveCase.
