src/helperTactics.v
@@ -1,26 +1,38 @@
-Require Import List.
+Require Import Arith Bool List ZArith.
+Local Open Scope Z_scope.
+
 
 Require Import wasmLite.
-Require Import wacket.
+Require Import language.definition.
+Require Import language.eval.
 Require Import compiler.
+Require Import utils.
 
-
-Ltac refineInductiveHypothesis := 
-match goal with 
-|   H0 : compile ?source = Succ ?compiled,
-    H1 : ?source d==> ?value,
-    IH : forall (compiled : wasmCode) (dupeResult : dupeResult),
-        compile ?source = Succ compiled ->
-        ?source d==> dupeResult -> _
-    |- _ => specialize ((IH compiled value) H0)
-|  H0: ?h1 -> ?h2, H1: ?h1 |- _ => specialize (H0 H1)
+Ltac refineHypothesis := 
+repeat match goal with 
+    | H : False |- _ => contradiction H
+    | H : _ \/ _ |- _ => destruct H
+    | H : _ /\ _ |- _ => destruct H
+    | H: ?a = ?a |- _ => clear H
+    | H: exists _, _ |- _ => destruct H
+    | H: (_,_) = (_,_) |- _ => inversion H;subst
+    | H: context[In _ _] |- _ => simpl in H
 end.
 
-Ltac logicAuto :=
-match goal with 
-| H: _ /\ _ |- _ => destruct H
-| H: _ \/ _ |- _ => destruct H
-| H: exists _, _ |- _ => destruct H
+Ltac copyHypothesis H := 
+    let tmp := fresh "H" in 
+    let eq := fresh "eq" in
+    remember H as tmp eqn: eq; clear eq
+.
+
+Ltac rewriteLeft := match goal with 
+| H: ?l = _ |- context[?l] => rewrite -> H
+| H: ?l = _, H0: context[?l] |- _ => rewrite -> H in H0
+| _ => fail
+end.
+Ltac rewriteRight := match goal with 
+| H: _ = ?r |- context[?r] => rewrite <- H
+| H: _ = ?r, H0: context[?r] |- _ => rewrite <- H in H0
 | _ => fail
 end.
 
@@ -38,4 +50,215 @@ Ltac removeListNils := match goal with
 | [H: context[_ ++ nil] |- _ ] => rewrite app_nil_r  in H
 | [H: context[nil ++ _] |- _ ] => rewrite app_nil_l  in H
 end.
+
+
+Ltac evalPreamble := 
+try match goal with 
+| |- forall (src : dupe) (val : dupeResult), src d==> (resultType val, val) -> _ => 
+        induction src; intros
+| |- forall (src : dupe) (val : dupeResult), evalDupe src = val -> _ =>
+        induction src; intros; try (simpl in *; subst; constructor)
+end.
+
+
+Ltac destructDupeProperties := 
+repeat match goal with 
+| dUniop: dupeUniaryOp |- _ => 
+        destruct dUniop; simpl in *;(try discriminate)
+| dResult: dupeResult |- _ => 
+        destruct dResult; simpl in *;(try discriminate)
+| dType: dupeType |- _ => 
+        destruct dType; simpl in *;(try discriminate)
+end.
+
+
+
+Ltac invertConstructiveDupe := 
+    match goal with 
+    | H: D_Integer ?z d==> (?type,?val) |- _ => inversion H; subst
+    | H: D_Boolean ?b d==> (?type,?val) |- _ => inversion H; subst
+    | H: (D_UniOp ?op ?src) d==> (?type,?val) |- _ => inversion H; subst
+    | H: (D_if ?srcIf ?srcThen ?srcElse) d==> (?type,?val) |- _ => inversion H; subst
+    end; (try reflexivity)
+.
+
+
+
+Theorem evalTypesSame:
+    forall src type val,
+        src d==> (type, val) ->
+        resultType val = type.
+Proof. 
+    induction src; intros;
+    evalPreamble;
+    destructDupeProperties;
+    invertConstructiveDupe;
+    refineHypothesis; (try discriminate);
+    repeat match goal with 
+    | H : ?src d==> (?type, ?val),
+        IH: forall (type : dupeType) (val : dupeResult),
+        ?src d==> (type, val) -> resultType val = type 
+        |- _ =>
+        specialize (IH type val H); subst
+    end; 
+    destructDupeProperties;
+    try reflexivity.
+Qed.
+
+Ltac removeSpecificType := 
+match goal with 
+    | |- forall (src : dupe) (type : dupeType) (val : dupeResult), src d==> (type, val) -> _ => 
+        intros; let tmp := fresh "H" in 
+        let eq := fresh "eq" in
+        match goal with 
+        | H: ?src d==> (?type, ?val) |- _ => 
+            remember H as tmp eqn: eq; clear eq;
+            apply evalTypesSame in tmp;
+            rewrite <- tmp in *; (try discriminate);
+            clear tmp; clear type;
+            generalize dependent val;
+            generalize dependent src
+        end
+    | H: ?src d==> (?type, ?val) |- _ => 
+        lazymatch goal with 
+        | H1: ?src1 d==> (type, ?val1),
+            H2: resultType ?val1 = type |- _ => fail
+        | H1: resultType val = type |- _ => fail
+        | |- _ => let tmp := fresh "H" in 
+            let eq := fresh "eq" in
+            remember H as tmp eqn: eq; clear eq;
+            apply evalTypesSame in tmp; 
+            rewrite <- tmp in *; (try discriminate)
+        end
+end.
+
+
+Ltac specializeIH := match goal with 
+|   IH: ?hyp -> ?prop, H: ?hyp |- _ => specialize (IH H)
+
+|   H: ?src d==> (?type, ?val),
+    IH: forall val : dupeResult, 
+    ?src d==> (resultType val, val) -> _ |- _ =>
+
+    let tmp := fresh "H" in 
+    let eq := fresh "eq" in
+    remember H as tmp eqn: eq; clear eq;
+    specialize (IH val);
+    eapply evalTypesSame in tmp; rewrite tmp in IH;
+    specialize (IH H);
+    clear tmp
+
+|   H0 : compile ?source = Succ ?compiled,
+    H1 : ?source d==> ?value,
+    IH : forall (compiled : wasmCode) (dupeResult : dupeResult),
+        compile ?source = Succ compiled ->
+        ?source d==> dupeResult -> _
+    |- _ => specialize ((IH compiled value) H0)
+
+|   IH: forall val: dupeResult,
+    evalDupe ?src = val -> _ |- _ => specialize (IH (evalDupe src))
+
+|   H: ?src d==> (resultType ?val, ?val),
+    IH: forall (val: dupeResult),
+    ?src d==> (resultType val, val) -> _ |- _ => specialize (IH val H)
+
+|   IH: ?a = ?a -> _ |- _ => 
+    let tmp := fresh "H" in 
+    assert (a = a) as tmp;[reflexivity | (specialize (IH tmp));clear tmp]
+| IH : resultType (evalDupe ?src) <> D_type_Error ->
+            ?src d==> (resultType (evalDupe ?src), evalDupe ?src)
+        |- _ => destruct (evalDupe src); simpl in IH; (try discriminate)
+|   IH: (?t1 <> ?t2) -> _ |-  _ => 
+    let tmp := fresh "H" in 
+    assert (t1 <> t2) as tmp;[
+        solve[discriminate]|
+        specialize (IH tmp); clear tmp
+    ]
+end.
+
+Ltac applyDupeEvalRule := 
+match goal with 
+    | |- (D_UniOp ?op ?src) d==> (?type, uniOpTransform ?op ?srcResult) => 
+        apply (E_D_UniOp src srcResult (resultType srcResult) op type); simpl;[
+            solve [try specializeIH; (try assumption)]| 
+            solve[(try contradiction);repeat ((left; reflexivity) || right)]
+        ]
+    | Hsrc1: ?src1 d==> (D_type_Int, DR_Int ?z),
+        Hsrc2: ?src2 d==> (?evalType, ?valThen),
+        Hsrc3: ?src3 d==> (?evalType, ?valElse)
+        |- (D_if ?src1 ?src2 ?src3) d==> (?evalType, ?valThen) => 
+            apply (E_D_ifInt src1 z src2 valThen src3 valElse evalType); assumption
+    | Hsrc1: ?src1 d==> (D_type_Bool, DR_Bool ?b),
+        Hsrc2: ?src2 d==> (?evalType, ?valThen),
+        Hsrc3: ?src3 d==> (?evalType, ?valElse)
+        |- (D_if ?src1 ?src2 ?src3) d==> (?evalType, if ?b then ?valThen else ?valElse) => 
+            destruct b; simpl; [
+                apply (E_D_ifTrue src1 src2 valThen src3 valElse evalType); assumption
+                | apply (E_D_ifFalse src1 src2 valThen src3 valElse evalType); assumption
+            ]  
+end.
+
+
+Ltac evalAuto := 
+    try removeSpecificType;
+    evalPreamble;
+    destructDupeProperties;
+    try invertConstructiveDupe;
+    refineHypothesis; (try discriminate);
+    destructDupeProperties;
+    repeat removeSpecificType;
+    repeat specializeIH; repeat rewriteLeft;
+    (try reflexivity);
+
+    try match goal with 
+    | H: _ = ?val |- _ d==> (_,?val) => rewrite <- H in *
+    end;
+    (simpl in *);
+    (try discriminate);
+    try applyDupeEvalRule;
+    try match goal with 
+    | H: (if ?b then _ else _) = _ |- _=> destruct b; discriminate
+    | H: D_type_Error <> D_type_Error |- _ => contradiction
+    end
+.
+
+Ltac stepCompletes := (
+    reflexivity || 
+    (apply Z.eqb_neq;reflexivity)
+).
+
+Ltac doesSingleStep := 
+    ( (eapply W_ST_64Const; stepCompletes)
+    || (eapply W_ST_32Const; stepCompletes)
+    || (eapply W_ST_inn_ibinop; stepCompletes)
+    || (eapply W_ST_inn_itestop; stepCompletes)
+    || (eapply W_ST_32IfTrue; stepCompletes)
+    || (eapply W_ST_32IfFalse; stepCompletes)
+    || (eapply W_ST_nop; stepCompletes)
+    || (eapply W_ST_unreachable; stepCompletes)
+    )
+.
+
+Ltac unfoldCommon :=
+    unfold testopOperation in *;
+    unfold binopOperation in *;
+    unfold uniOpTransform in *;
+    unfold compileUniOp in *
+.
+
+
+Ltac doesStep :=
+repeat (
+    unfoldCommon;
+    simpl in *;
+    (repeat destructBools);
+    (repeat removeListNils); 
+    (try assumption);
+    (try discriminate);
+    match goal with 
+    | [|- _ w-->* _ ]=> econstructor
+    | [|- multi wasmStepInd _ _] => econstructor
+    | [|- _ w--> _] => doesSingleStep
+    end
+).
 
