src/language/eval.v
@@ -1,0 +1,74 @@
+Require Import Bool List ZArith.
+
+Local Open Scope Z_scope.
+
+Require Import definition.
+
+Inductive dupeResult : Type :=
+| DR_Int: Z -> dupeResult
+| DR_Bool: bool -> dupeResult
+| DR_Error: dupeResult
+.
+
+Definition resultType result := match result with 
+| DR_Int _ => D_type_Int
+| DR_Bool _ => D_type_Bool
+| DR_Error => D_type_Error
+end.
+
+
+Definition uniOpTransform op result := match (op, result) with 
+| (D_U_add1, DR_Int z) => DR_Int (z + 1)
+| (D_U_sub1, DR_Int z) => DR_Int (z - 1)
+| (D_U_zero, DR_Int z) => DR_Bool (z =? 0)
+| (D_U_not, DR_Bool b) => DR_Bool (negb b)
+| _ => DR_Error
+end.
+
+
+Fixpoint evalDupe(d : dupe) := match d with 
+| (D_Integer z) => (DR_Int z)
+| (D_Boolean b) => (DR_Bool b)
+| (D_UniOp op exp) => uniOpTransform op (evalDupe exp)
+| (D_if e1 e2 e3) => match (evalDupe e1, evalDupe e2, evalDupe e3) with 
+    | (DR_Bool b, res1, res2) => 
+        if (typeSame (resultType res1) (resultType res2)) && (negb (typeSame (resultType res1) D_type_Error))
+        then if b then res1 else res2
+        else DR_Error
+    | (DR_Int _, res1, res2 ) =>
+        if (typeSame (resultType res1) (resultType res2)) && (negb (typeSame (resultType res1) D_type_Error))
+        then res1
+        else DR_Error
+    | _ => DR_Error
+    end
+end.
+
+
+(* this will probably have to be changed because of how integers are represented in binary*)
+Reserved Notation " src 'd==>' val " (at level 50, left associativity).
+Inductive dupeEval: dupe -> (dupeType * dupeResult)%type -> Prop :=
+| E_D_Interger: forall z, (D_Integer z) d==> (D_type_Int, (DR_Int z))
+| E_D_Boolean: forall b, (D_Boolean b) d==> (D_type_Bool ,(DR_Bool b))
+
+| E_D_UniOp: forall t v inputType op evalType,
+    t d==> (inputType, v) ->
+    In (inputType, evalType) (uniOpTypeSignature op) ->
+    (D_UniOp op t) d==> (evalType,(uniOpTransform op v))
+
+| E_D_ifFalse: forall t_if t_then vt t_else ve evalType,
+    t_if d==> (D_type_Bool,(DR_Bool false)) -> 
+    t_then d==> (evalType,vt) ->
+    t_else d==> (evalType,ve) ->
+    (D_if t_if t_then t_else) d==> (evalType,ve)
+| E_D_ifTrue: forall t_if t_then vt t_else ve evalType,
+    t_if d==> (D_type_Bool,(DR_Bool true)) -> 
+    t_then d==> (evalType,vt) ->
+    t_else d==> (evalType,ve) ->
+    (D_if t_if t_then t_else) d==> (evalType,vt)
+| E_D_ifInt: forall t_if z t_then vt t_else ve evalType,
+    t_if d==> (D_type_Int,(DR_Int z)) -> 
+    t_then d==> (evalType,vt) ->
+    t_else d==> (evalType,ve) ->
+    (D_if t_if t_then t_else) d==> (evalType,vt)
+
+where " src 'd==>' val " := (dupeEval src val).
