src/language/properties.v
@@ -1,0 +1,63 @@
+Require Import definition.
+Require Import eval.
+
+Require Import helperTactics.
+
+Require Import List.
+
+
+Theorem TypeOfDupe_same_as_Eval:
+    forall src type val,
+        src d==> (type, val) -> 
+        typeOfDupe src = type.
+Proof.
+    evalAuto.
+Qed.
+    
+
+Theorem evalDupe_implies_dupeEval: 
+    forall src val,
+    evalDupe src = val ->
+    ((resultType val) <> D_type_Error) ->
+    src d==> (resultType val, val).
+Proof.
+    evalAuto.
+Qed.
+
+
+Theorem dupeEval_implies_evalDupe: 
+    forall src val,
+    src d==> (resultType val, val) ->
+    evalDupe src = val.
+Proof.
+    evalAuto.
+Qed.
+
+
+Theorem dupeNotEvalError:
+forall src val,
+    src d==> (resultType val, val) ->
+    ((resultType val) <> D_type_Error).
+Proof.
+    evalAuto.
+Qed.
+
+
+Theorem evalEquivalence: 
+    forall src val,
+    src d==> (resultType val, val) <-> ((evalDupe src = val) /\ ((resultType val) <> D_type_Error)).
+Proof.
+    intros. 
+    split.
+    - split.
+        + apply dupeEval_implies_evalDupe. assumption.
+        + apply (dupeNotEvalError src). assumption.
+    - intros. 
+        destruct H.
+        apply  evalDupe_implies_dupeEval.
+        + assumption.
+        + assumption.
+Qed.
+
+
+
